Simplify the TwoDisk/OneDisk module hierarchy.

src/Examples/ReplicatedDisk/OneDiskAPI.v
@@ -1,27 +1,40 @@
 Require Import POCS.
 Require Export Maybe Disk.
 
-Definition State := disk.
 
-Inductive OneDiskOp : Type -> Type :=
-| op_read (a : addr) : OneDiskOp block
-| op_write (a : addr) (b : block) : OneDiskOp unit
-| op_size : OneDiskOp nat.
+Module OneDisk.
 
-Inductive one_disk_op_step : OpSemantics OneDiskOp State :=
-| step_read : forall a r state,
-    match diskGet state a with
-    | Some b0 => r = b0
-    | None => exists b, r = b
-    end ->
-    one_disk_op_step (op_read a) state state r
-| step_write : forall a b state state',
-    state' = (diskUpd state a b) ->
-    one_disk_op_step (op_write a b) state state' tt
-| step_size : forall state,
-    one_disk_op_step (op_size) state state (diskSize state).
+  Definition State := disk.
+  Inductive Op : Type -> Type :=
+  | op_read (a : addr) : Op block
+  | op_write (a : addr) (b : block) : Op unit
+  | op_size : Op nat.
 
-Definition read_spec (a : addr) : Specification block unit State :=
+  Inductive op_step : OpSemantics Op State :=
+  | step_read : forall a r state,
+      match diskGet state a with
+      | Some b0 => r = b0
+      | None => exists b, r = b
+      end ->
+      op_step (op_read a) state state r
+  | step_write : forall a b state state',
+      state' = (diskUpd state a b) ->
+      op_step (op_write a b) state state' tt
+  | step_size : forall state,
+      op_step (op_size) state state (diskSize state).
+
+  Inductive one_disk_failure : CrashSemantics State :=
+  | step_id : forall (state: State), one_disk_failure state state tt.
+
+  Definition ODBaseDynamics : Dynamics Op State :=
+    {| step := op_step; crash_step := one_disk_failure |}.
+
+  Definition ODLayer : Layer Op :=
+    {| Layer.State := State; sem := ODBaseDynamics; initP := fun _ => True |}.
+
+End OneDisk.
+
+Definition read_spec (a : addr) : Specification block unit OneDisk.State :=
   fun state => {|
     pre := True;
     post := fun state' r =>
@@ -31,7 +44,7 @@ Definition read_spec (a : addr) : Specification block unit State :=
       state' = state
   |}.
 
-Definition write_spec (a : addr) (v : block) : Specification _ unit State :=
+Definition write_spec (a : addr) (v : block) : Specification _ unit OneDisk.State :=
   fun state => {|
     pre := True;
     post := fun state' r =>
@@ -40,7 +53,7 @@ Definition write_spec (a : addr) (v : block) : Specification _ unit State :=
       state' = state \/ state' = diskUpd state a v
   |}.
 
-Definition size_spec : Specification nat unit State :=
+Definition size_spec : Specification nat unit OneDisk.State :=
   fun state => {|
     pre := True;
     post := fun state' r =>
@@ -48,13 +61,3 @@ Definition size_spec : Specification nat unit State :=
     alternate := fun state' r =>
       state' = state
   |}.
-
-Inductive one_disk_failure : CrashSemantics State :=
-| step_id : forall (state: State), one_disk_failure state state tt.
-
-Definition ODBaseDynamics : Dynamics OneDiskOp State :=
-  {| step := one_disk_op_step; crash_step := one_disk_failure |}.
-
-Definition ODLayer : Layer OneDiskOp :=
-  {| Layer.State := State; sem := ODBaseDynamics; initP := fun _ => True |}.
-
