src/Examples/ReplicatedDisk/TwoDiskAPI.v
@@ -1,111 +1,128 @@
 Require Import POCS.
 Require Export Maybe.
-Require Export TwoDiskBaseAPI.
+Require Export Disk.
+
+Import RelationNotations.
 
 (**
-TwoDiskAPI supports reading and writing to two disks, with the possibility for a
-disk to fail at any time. This layer provides easier-to-use specifications
-written in terms of [maybe_holds] (the ?|= notation). The fact that at least one
-disk is always functioning is encoded in the inductive type [TwoDiskBaseAPI.State]
-itself; it has only three cases, for both disks, only disk 0, and only disk 1.
+TwoDiskAPI supports reading and writing to two disks. It also allows one
+disk to fail at any time (just before any operation). Note that disk failure is
+separate from program crashes: programs can still crash and recover. In this
+model, there is no way to recover from a disk failure (that is, we have a
+fail-stop model).
+
 *)
 
+Module TwoDisk.
+  Inductive diskId :=
+  | d0
+  | d1.
 
-Definition other (i : diskId) :=
-  match i with
-  | d0 => d1
-  | d1 => d0
-  end.
+  Inductive DiskResult T :=
+  | Working (v:T)
+  | Failed.
 
-Definition read_spec (i : diskId) (a : addr) : _ -> Specification _ (unit) State :=
-  fun '(d, F) state => {|
-    pre :=
-      get_disk i         state ?|= eq d /\
-      get_disk (other i) state ?|= F;
-    post := fun state' r =>
-      match r with
-      | Working v =>
-        get_disk i         state' ?|= eq d /\
-        get_disk (other i) state' ?|= F /\
-        diskGet d a ?|= eq v
-      | Failed =>
-        get_disk i         state' ?|= missing /\
-        get_disk (other i) state' ?|= F
-      end;
-    alternate := fun state' r =>
-      get_disk i         state' ?|= eq d /\
-      get_disk (other i) state' ?|= F;
-  |}.
+  Arguments Failed {T}.
 
-Definition write_spec (i : diskId) (a : addr) (b : block) : _ -> Specification (DiskResult unit) unit _ :=
-  fun '(d, F) state => {|
-    pre :=
-      get_disk i         state ?|= eq d /\
-      get_disk (other i) state ?|= F;
-    post := fun state' r =>
-      match r with
-      | Working _ =>
-        get_disk i         state' ?|= eq (diskUpd d a b) /\
-        get_disk (other i) state' ?|= F
-      | Failed =>
-        get_disk i         state' ?|= missing /\
-        get_disk (other i) state' ?|= F
-      end;
-    alternate := fun state' _ =>
-      (get_disk i state' ?|= eq d \/
-       get_disk i state' ?|= eq (diskUpd d a b) /\ a < diskSize d) /\
-      get_disk (other i) state' ?|= F;
-  |}.
+  Inductive State :=
+  | BothDisks (d_0:disk) (d_1:disk)
+  | OnlyDisk0 (d_0:disk)
+  | OnlyDisk1 (d_1:disk).
 
-Definition size_spec (i : diskId) : _ -> Specification _ unit _ :=
-  fun '(d, F) state => {|
-    pre :=
-      get_disk i         state ?|= eq d /\
-      get_disk (other i) state ?|= F;
-    post := fun state' r =>
-      match r with
-      | Working n =>
-        get_disk i         state' ?|= eq d /\
-        get_disk (other i) state' ?|= F /\
-        n = diskSize d
-      | Failed =>
-        get_disk i         state' ?|= missing /\
-        get_disk (other i) state' ?|= F
-      end;
-    alternate := fun state' _ =>
-      get_disk i         state' ?|= eq d /\
-      get_disk (other i) state' ?|= F;
-  |}.
+  Definition disk0 (state:State) : option disk :=
+    match state with
+    | BothDisks d_0 _ => Some d_0
+    | OnlyDisk0 d => Some d
+    | OnlyDisk1 _ => None
+    end.
 
+  Definition disk1 (state:State) : option disk :=
+    match state with
+    | BothDisks _ d_1 => Some d_1
+    | OnlyDisk0 _ => None
+    | OnlyDisk1 d => Some d
+    end.
 
-Module Type TwoDiskAPI.
+  Definition get_disk (i:diskId) (state:State) : option disk :=
+    match i with
+    | d0 => disk0 state
+    | d1 => disk1 state
+    end.
 
-  (*
-  Axiom init : proc InitResult.
-   *)
-  
-  Axiom read : diskId -> addr -> proc Op (DiskResult block).
-  Axiom write : diskId -> addr -> block -> proc Op (DiskResult unit).
-  Axiom size : diskId -> proc Op (DiskResult nat).
-  Axiom recover : proc Op unit.
+  Definition set_disk (i:diskId) (state:State) (d:disk) : State :=
+    match i with
+    | d0 => match state with
+            | BothDisks _ d_1 => BothDisks d d_1
+            | OnlyDisk0 _ => OnlyDisk0 d
+            | OnlyDisk1 d_1 => BothDisks d d_1
+            end
+    | d1 => match state with
+            | BothDisks d_0 _ => BothDisks d_0 d
+            | OnlyDisk0 d_0 => BothDisks d_0 d
+            | OnlyDisk1 _ => OnlyDisk1 d
+            end
+    end.
 
-  (*
-  Axiom abstr : Abstraction State.
-   *)
+  Inductive Op : Type -> Type :=
+  | op_read (i : diskId) (a : addr) : Op (DiskResult block)
+  | op_write (i : diskId) (a : addr) (b : block) : Op (DiskResult unit)
+  | op_size (i : diskId) : Op (DiskResult nat).
 
-  (*
-  Axiom init_ok : init_abstraction init recover abstr inited_any.
-   *)
+  Inductive op_step : OpSemantics Op State :=
+  | step_read : forall a i r state,
+      match get_disk i state with
+      | Some d => match diskGet d a with
+                  | Some b0 => r = Working b0
+                  | None => exists b, r = Working b
+                  end
+      | None => r = Failed
+      end ->
+      op_step (op_read i a) state state r
+  | step_write : forall a i b state r state',
+      match get_disk i state with
+      | Some d => state' = set_disk i state (diskUpd d a b) /\
+                  r = Working tt
+      | None => r = Failed /\ state' = state
+      end ->
+      op_step (op_write i a b) state state' r
+  | step_size : forall i state r,
+      match get_disk i state with
+      | Some d => r = Working (diskSize d)
+      | None => r = Failed
+      end ->
+      op_step (op_size i) state state r.
 
-  Axiom read_ok : forall i a dF, proc_cspec TDBaseDynamics (read i a) (read_spec i a dF).
-  Axiom write_ok : forall i a v dF, proc_cspec TDBaseDynamics (write i a v) (write_spec i a v dF).
-  Axiom size_ok : forall i dF, proc_cspec TDBaseDynamics (size i) (size_spec i dF).
-  Axiom recover_noop : rec_noop TDBaseDynamics recover eq.
+  Inductive bg_failure : State -> State -> unit -> Prop :=
+  | step_id : forall (state: State), bg_failure state state tt
+  | step_fail0 : forall d_0 d_1,
+      bg_failure (BothDisks d_0 d_1) (OnlyDisk1 d_1) tt
+  | step_fail1 : forall d_0 d_1,
+      bg_failure (BothDisks d_0 d_1) (OnlyDisk0 d_0) tt.
 
-  Hint Resolve init_ok.
-  Hint Resolve read_ok.
-  Hint Resolve write_ok.
-  Hint Resolve size_ok.
-  Hint Resolve recover_noop.
+  Definition pre_step {opT State}
+             (bg_step: State -> State -> unit -> Prop)
+             (step: OpSemantics opT State) :
+    OpSemantics opT State :=
+    fun T (op: opT T) state state'' v =>
+      exists state', bg_step state state' tt /\
+                     step _ op state' state'' v.
 
-End TwoDiskAPI.
+  Definition combined_step := pre_step bg_failure (@op_step).
+
+  Definition TDBaseDynamics : Dynamics Op State :=
+    {| step := op_step; crash_step := RelationAlgebra.identity |}.
+
+  Definition td_init (s: State) :=
+    exists d_0' d_1',
+      disk0 s ?|= eq d_0' /\
+      disk1 s ?|= eq d_1'.
+
+  Definition TDLayer : Layer Op :=
+    {| Layer.State := State; sem := TDBaseDynamics; initP := td_init |}.
+End TwoDisk.
+
+(* Wrappers around the primitive operations *)
+Import TwoDisk.
+Definition read i a : proc Op (DiskResult block) := Prim (op_read i a).
+Definition write i a b : proc Op (DiskResult unit) := Prim (op_write i a b).
+Definition size i : proc Op (DiskResult nat) := Prim (op_size i).
